noclock/solution_basebound/scratch.lean
@@ -1,0 +1,5 @@
+opaque N : Nat
+axiom hN : 0 < N
+
+def test (x : Fin N) : Fin N :=
+  x + ⟨1 % N, Nat.mod_lt 1 hN⟩
